autoclrs/ch06-heapsort/c/CLRS.Ch06.Heap.C.BridgeLemmas.fst
@@ -8,6 +8,7 @@ module CLRS.Ch06.Heap.C.BridgeLemmas
 open CLRS.Ch06.Heap.Spec
 open CLRS.Ch06.Heap.Lemmas
 module Seq  = FStar.Seq
+module SeqP = FStar.Seq.Properties
 module I32  = FStar.Int32
 module SZ   = FStar.SizeT
 module Classical = FStar.Classical
@@ -20,6 +21,72 @@ let extract_ints (s: Seq.seq (option I32.t)) (n: nat{all_some s n})
   : Tot (r: Seq.seq int{Seq.length r == n /\
     (forall (i: nat). i < n ==> Seq.index r i == I32.v (Some?.v (Seq.index s i)))})
   = Seq.init n (fun (i: nat{i < n}) -> (I32.v (Some?.v (Seq.index s i)) <: int))
+
+// ================================================================
+// Permutation lemmas for option Int32.t sequences
+// ================================================================
+
+let option_perm_refl (s: Seq.seq (option I32.t))
+  : Lemma (SeqP.permutation (option I32.t) s s)
+  = ()
+
+let option_perm_trans (s1 s2 s3: Seq.seq (option I32.t))
+  : Lemma
+    (requires SeqP.permutation (option I32.t) s1 s2 /\
+              SeqP.permutation (option I32.t) s2 s3)
+    (ensures SeqP.permutation (option I32.t) s1 s3)
+  = ()
+
+#push-options "--z3rlimit 40 --fuel 1 --ifuel 0"
+
+let swap_option_seq_eq (s: Seq.seq (option I32.t))
+  (i j: nat{i < Seq.length s /\ j < Seq.length s /\ i <> j})
+  : Lemma
+    (Seq.equal
+      (Seq.upd (Seq.upd s i (Seq.index s j)) j (Seq.index s i))
+      (SeqP.swap s i j))
+  = ()
+
+#pop-options
+
+private let rec count_ext (#a: eqtype) (x: a) (s1 s2: Seq.seq a)
+  : Lemma
+    (requires Seq.equal s1 s2)
+    (ensures SeqP.count x s1 = SeqP.count x s2)
+    (decreases Seq.length s1)
+  = if Seq.length s1 = 0 then ()
+    else count_ext x (Seq.tail s1) (Seq.tail s2)
+
+private let perm_ext (#a: eqtype) (s1 s2 s3: Seq.seq a)
+  : Lemma
+    (requires SeqP.permutation a s1 s2 /\ Seq.equal s2 s3)
+    (ensures SeqP.permutation a s1 s3)
+  = let aux (x: a) : Lemma (SeqP.count x s1 = SeqP.count x s3) =
+      count_ext x s2 s3
+    in
+    Classical.forall_intro aux
+
+#push-options "--z3rlimit 40 --fuel 1 --ifuel 0"
+
+let swap_option_perm (s: Seq.seq (option I32.t))
+  (i j: nat{i < Seq.length s /\ j < Seq.length s})
+  : Lemma (SeqP.permutation (option I32.t) s
+    (Seq.upd (Seq.upd s i (Seq.index s j)) j (Seq.index s i)))
+  = if i = j then begin
+      assert (Seq.equal s (Seq.upd (Seq.upd s i (Seq.index s j)) j (Seq.index s i)));
+      perm_ext s s (Seq.upd (Seq.upd s i (Seq.index s j)) j (Seq.index s i))
+    end
+    else begin
+      let lo = if i <= j then i else j in
+      let hi = if i <= j then j else i in
+      SeqP.lemma_swap_permutes #(option I32.t) s lo hi;
+      assert (Seq.equal (SeqP.swap s lo hi) (SeqP.swap s i j));
+      perm_ext s (SeqP.swap s lo hi) (SeqP.swap s i j);
+      swap_option_seq_eq s i j;
+      perm_ext s (SeqP.swap s i j) (Seq.upd (Seq.upd s i (Seq.index s j)) j (Seq.index s i))
+    end
+
+#pop-options
 
 // ================================================================
 // root_ge_element_bridge
